generational/spec/GC.Gen.CheneyBFS.fsti
@@ -72,25 +72,25 @@ val fwd_well_formed_covers_reachable
 
 val forward_one_fwd_monotone
   (minor: minor_state) (cs: CheneySpec.cheney_state) (addr: U64.t) (x: U64.t)
-  : Lemma (requires cs.cs_fwd x <> 0UL)
+  : Lemma (requires cs.cs_fwd x <> 0UL /\ minor_infix_wf minor)
           (ensures (CheneySpec.cheney_forward_one minor cs addr).cs_fwd x <> 0UL)
 
 val forward_fields_fwd_monotone
   (minor: minor_state) (cs: CheneySpec.cheney_state)
   (parent: U64.t) (idx: nat) (wosize: nat) (x: U64.t)
-  : Lemma (requires cs.cs_fwd x <> 0UL)
+  : Lemma (requires cs.cs_fwd x <> 0UL /\ minor_infix_wf minor)
           (ensures (CheneySpec.cheney_forward_fields minor cs parent idx wosize).cs_fwd x <> 0UL)
 
 val forward_roots_fwd_monotone
   (minor: minor_state) (cs: CheneySpec.cheney_state)
   (roots: seq U64.t) (idx: nat) (x: U64.t)
-  : Lemma (requires cs.cs_fwd x <> 0UL)
+  : Lemma (requires cs.cs_fwd x <> 0UL /\ minor_infix_wf minor)
           (ensures (CheneySpec.cheney_forward_roots minor cs roots idx).cs_fwd x <> 0UL)
 
 val scan_fwd_monotone
   (minor: minor_state) (cs: CheneySpec.cheney_state)
   (scan: nat) (fuel: nat) (x: U64.t)
-  : Lemma (requires cs.cs_fwd x <> 0UL)
+  : Lemma (requires cs.cs_fwd x <> 0UL /\ minor_infix_wf minor)
           (ensures (CheneySpec.cheney_scan minor cs scan fuel).cs_fwd x <> 0UL)
 
 /// ---------------------------------------------------------------------------
